Complete proof that non-touching PseudoC actions commute.
This then guarantees that graphs built with them will indeed evaluate
deterministically.

hol/PseudoCPropsScript.sml
@@ -5,6 +5,8 @@ open lcsymtacs
 open bagTheory
 open PseudoCTheory
 open actionGraphTheory
+open pred_setTheory finite_mapTheory
+open intLib
 
 val _ = new_theory "PseudoCProps";
 
@@ -16,8 +18,8 @@ val _ = export_rewrites ["expr_weight_def"]
 
 val dexpr_weight_def = Define`
   (dexpr_weight (DValue v) = 0:num) ∧
-  (dexpr_weight (Read v e) = 1 + expr_weight e) ∧
-  (dexpr_weight (Convert e) = expr_weight e)
+  (dexpr_weight (ARead v e) = 1 + expr_weight e) ∧
+  (dexpr_weight (VRead v) = 1)
 `;
 val _ = export_rewrites ["dexpr_weight_def"]
 
@@ -81,27 +83,27 @@ val transitive_LT = store_thm(
   simp[relationTheory.transitive_def]);
 
 
-val SUM_IMAGE_CONG = REWRITE_RULE [GSYM AND_IMP_INTRO] pred_setTheory.SUM_IMAGE_CONG
+val SUM_IMAGE_CONG = REWRITE_RULE [GSYM AND_IMP_INTRO] SUM_IMAGE_CONG
 val BAG_CARD_SUM_IMAGE = store_thm(
   "BAG_CARD_SUM_IMAGE",
   ``FINITE_BAG b ==>
     (BAG_CARD b = SUM_IMAGE b { e | BAG_IN e b })``,
   Q.ID_SPEC_TAC `b` THEN Induct_on `FINITE_BAG` THEN
-  SRW_TAC [][pred_setTheory.SUM_IMAGE_THM, BAG_CARD_THM] THEN
-  SIMP_TAC (srw_ss()) [BAG_INSERT, pred_setTheory.GSPEC_OR] THEN
+  SRW_TAC [][SUM_IMAGE_THM, BAG_CARD_THM] THEN
+  SIMP_TAC (srw_ss()) [BAG_INSERT, GSPEC_OR] THEN
   `{ e | BAG_IN e b} = SET_OF_BAG b`
-    by SRW_TAC [][SET_OF_BAG, pred_setTheory.EXTENSION] THEN
-  SRW_TAC[][pred_setTheory.SUM_IMAGE_UNION,
-            pred_setTheory.SUM_IMAGE_THM] THEN
+    by SRW_TAC [][SET_OF_BAG, EXTENSION] THEN
+  SRW_TAC[][SUM_IMAGE_UNION,
+            SUM_IMAGE_THM] THEN
   Cases_on `e IN SET_OF_BAG b` THENL [
-    SRW_TAC[][pred_setTheory.INSERT_INTER, pred_setTheory.SUM_IMAGE_THM] THEN
+    SRW_TAC[][INSERT_INTER, SUM_IMAGE_THM] THEN
     `SET_OF_BAG b = e INSERT (SET_OF_BAG b DELETE e)`
-      by (SRW_TAC[][pred_setTheory.EXTENSION] THEN METIS_TAC[IN_SET_OF_BAG])THEN
+      by (SRW_TAC[][EXTENSION] THEN METIS_TAC[IN_SET_OF_BAG])THEN
     POP_ASSUM (fn th => ONCE_REWRITE_TAC [th]) THEN
-    SRW_TAC [][pred_setTheory.SUM_IMAGE_THM] THEN
+    SRW_TAC [][SUM_IMAGE_THM] THEN
     SRW_TAC[ARITH_ss][] THEN
     SRW_TAC[][Cong SUM_IMAGE_CONG],
-    SRW_TAC [][pred_setTheory.INSERT_INTER, pred_setTheory.SUM_IMAGE_THM] THEN
+    SRW_TAC [][INSERT_INTER, SUM_IMAGE_THM] THEN
     `!x. x IN SET_OF_BAG b ==> x <> e` by METIS_TAC[] THEN
     SRW_TAC[][Cong SUM_IMAGE_CONG] THEN
     `b e = 0` suffices_by SRW_TAC[ARITH_ss][] THEN
@@ -132,12 +134,11 @@ val eval_terminates = store_thm(
   "eval_terminates",
   ``∀a b. eval a b ⇒ inv_image (mlt (<) LEX (<)) (λ(m,lm,s). (loopbag s, stmt_weight s)) b a``,
   Induct_on `eval a b` >> rpt strip_tac >>
-  lfs[pairTheory.LEX_DEF, pred_setTheory.MAX_SET_THM]
+  lfs[pairTheory.LEX_DEF, MAX_SET_THM, listTheory.SUM_APPEND]
   >- (Cases_on `b` >> simp[])
   >- (simp[mltLT_SING0] >> metis_tac[])
   >- (Cases_on `expr` >> fs[isValue_def])
-  >- (simp[listTheory.SUM_APPEND] >> Cases_on `expr` >> fs[isValue_def])
-  >- simp[listTheory.SUM_APPEND]
+  >- (Cases_on `expr` >> fs[isValue_def])
   >- simp[rich_listTheory.FOLDR_MAP, mlt_loopbag_lemma]
   >- (simp[mltLT_SING0] >> metis_tac[])
   >- simp[rich_listTheory.FOLDR_MAP, mlt_loopbag_lemma]
@@ -157,7 +158,8 @@ val eval_terminates = store_thm(
    ---------------------------------------------------------------------- *)
 
 val gtouches_def = Define`
-  gtouches g1 g2 <=> ∃a1 a2. a1 ∈ g1 ∧ a2 ∈ g2 ∧ touches a1 a2
+  gtouches (g1:(α,β,γ)action_graph) (g2:(α,β,γ)action_graph) ⇔
+    ∃a1 a2. a1 ∈ g1 ∧ a2 ∈ g2 ∧ touches a1 a2
 `;
 
 open monadsyntax
@@ -168,13 +170,12 @@ val _ = overload_on ("assert", ``OPTION_GUARD``)
 (* opt_sequence : (α option) list -> α list option *)
 val OPT_SEQUENCE_def = Define`
   (OPT_SEQUENCE [] = SOME []) ∧
-  (OPT_SEQUENCE (NONE :: _) = NONE) ∧
-  (OPT_SEQUENCE (SOME x :: rest) = OPTION_MAP (CONS x) (OPT_SEQUENCE rest))
+  (OPT_SEQUENCE (h :: t) = lift2 CONS h (OPT_SEQUENCE t))
 `;
 
 val MEM_FOLDR_mlt = store_thm(
   "MEM_FOLDR_mlt",
-  ``MEM e l ==>
+  ``MEM e l ⇒
     mlt $< (loopbag (f e)) (FOLDR (\e a. loopbag (f e) ⊎ a) {|0|} l) ∨
     loopbag (f e) = FOLDR (\e a. loopbag (f e) ⊎ a) {|0|} l``,
   Induct_on `l` >> dsimp[] >> rpt strip_tac >> res_tac
@@ -187,32 +188,48 @@ val MEM_FOLDR_mlt = store_thm(
 
 val pushG_def = Define`pushG v = imap (λi. v::i)`
 
+val _ = Datatype`actionRW = Array aname int | Variable vname`
+
+val actRWName_def = Define`
+  (actRWName (Array a _) = a) ∧
+  (actRWName (Variable v) = v)
+`;
+val _ = export_rewrites ["actRWName_def"]
+
+val lookupRW_def = Define`
+  (lookupRW m (Array a i) = lookup_array m a i) ∧
+  (lookupRW m (Variable v) = lookup_v m v)
+`;
+
 val getReads_def = Define`
   (getReads m [] = SOME []) ∧
-  (getReads m (Read vname i_e :: des) =
-     lift2 (λi rest. (vname,i) :: rest)
+  (getReads m (ARead aname i_e :: des) =
+     lift2 (λi rest. Array aname i :: rest)
            (some i. evalexpr m i_e = Int i)
-           (getReads m des))
+           (getReads m des)) ∧
+  (getReads m (VRead vname :: des) =
+     OPTION_MAP (CONS (Variable vname)) (getReads m des)) ∧
+  (getReads m (DValue _ :: des) = getReads m des)
 `;
 
 val mergeReads0_def = Define`
-  (mergeReads0 m [] acc opn vs = opn (REVERSE acc)) ∧
-  (mergeReads0 m (Convert e :: ds) acc opn vs =
-     mergeReads0 m ds (evalexpr m e :: acc) opn vs) ∧
-  (mergeReads0 m (DValue v :: ds) acc opn vs =
-     mergeReads0 m ds (v :: acc) opn vs) ∧
-  (mergeReads0 m (Read _ _ :: ds) acc opn vs =
-     mergeReads0 m ds (HD vs :: acc) opn (TL vs))
+  (mergeReads0 [] acc opn vs = opn (REVERSE acc)) ∧
+  (mergeReads0 (VRead _ :: ds) acc opn vs =
+     mergeReads0 ds (HD vs :: acc) opn (TL vs)) ∧
+  (mergeReads0 (DValue v :: ds) acc opn vs =
+     mergeReads0 ds (v :: acc) opn vs) ∧
+  (mergeReads0 (ARead _ _ :: ds) acc opn vs =
+     mergeReads0 ds (HD vs :: acc) opn (TL vs))
 `;
 
 val mergeReads_def = Define`
-  mergeReads m ds opn = mergeReads0 m ds [] opn
+  mergeReads ds opn = mergeReads0 ds [] opn
 `;
 
 val evalDexpr_def = Define`
-  (evalDexpr m (Convert e) = SOME (evalexpr m e)) ∧
   (evalDexpr m (DValue v) = SOME v) ∧
-  (evalDexpr m (Read aname e_i) =
+  (evalDexpr m (VRead vname) = SOME (lookup_v m vname)) ∧
+  (evalDexpr m (ARead aname e_i) =
      do
        i <- (some i. evalexpr m e_i = Int i);
        SOME (lookup_array m aname i)
@@ -224,9 +241,468 @@ val stackInc_def = Define`
   (stackInc (h::t) = h + 1n :: t)
 `;
 
+val ap1_def = Define`ap1 f (x,y) = (f x, y)`;
+val ap2_def = Define`ap2 f (x,y) = (x, f y)`;
 val ap3_def = Define`
   ap3 f (x,y,z) = (x,y,f z)
 `;
+val _ = export_rewrites ["ap1_def", "ap2_def", "ap3_def"]
+
+val selapf_def = Define`
+  selapf a lm =
+    if actRWName a.write ∈ FDOM lm then
+      (FST : memory # memory -> memory,
+       ap1 : (memory -> memory) -> memory # memory -> memory # memory)
+    else (SND, ap2)
+`;
+
+val updf_def = Define`
+  updf w value m =
+    case w of
+      | Array a i => upd_array m a i value
+      | Variable vnm => case FLOOKUP m vnm of
+                          NONE => NONE
+                        | SOME (Array _) => NONE
+                        | SOME _ => if ∀els. value ≠ Array els then
+                                      SOME(m |+ (vnm, value))
+                                    else NONE
+`;
+
+val apply_action_def = Define`
+  apply_action a lmm_opt =
+    do
+      (lm,m) <- lmm_opt;
+      vs <- SOME(MAP (lookupRW (lm ⊌ m)) a.reads);
+      (self,apf) <- SOME (selapf a lm);
+      value <- SOME (a.expr vs);
+      m' <- updf a.write value (self (lm,m));
+      SOME(apf (K m') (lm,m))
+    od
+`;
+
+val lift_OPTION_BIND = store_thm(
+  "lift_OPTION_BIND",
+  ``OPTION_BIND (OPTION_BIND v f) g =
+    OPTION_BIND v (combin$C (OPTION_BIND o f) g)``,
+  Cases_on `v` >> simp[]);
+
+val updf_EQ_NONE = store_thm(
+  "updf_EQ_NONE",
+  ``updf w value m = NONE ⇔
+     (∃a i. w = Array a i ∧ upd_array m a i value = NONE) ∨
+     ∃vnm. w = Variable vnm ∧ (vnm ∉ FDOM m ∨ (∃els. value = Array els) ∨
+                               vnm ∈ FDOM m ∧ ∃els. m ' vnm = Array els)``,
+  Cases_on `w` >> simp[updf_def] >>
+  rw[FLOOKUP_DEF] >> fs[] >> Cases_on `m ' s` >> simp[]) ;
+
+val updarray_EQ_NONE = store_thm(
+  "updarray_EQ_NONE",
+  ``upd_array m a i v = NONE ⇔
+    ∀vlist. FLOOKUP m a = SOME (Array vlist) ⇒ i < 0 ∨ &LENGTH vlist ≤ i``,
+  `FLOOKUP m a = NONE ∨ ∃v'. FLOOKUP m a = SOME v'`
+    by metis_tac[optionTheory.option_CASES] >>
+  simp[upd_array_def] >> Cases_on `v'` >> simp[]);
+
+val updf_preserves_FDOMs = store_thm(
+  "updf_preserves_FDOMs",
+  ``updf w value m = SOME m' ⇒ FDOM m' = FDOM m``,
+  Cases_on `w` >> simp[updf_def, upd_array_def] >> rw[] >>
+  simp[ABSORPTION_RWT] >>
+  Cases_on `FLOOKUP m s` >> fs[] >>
+  Cases_on `x` >> fs[] >> rw[] >>
+  match_mp_tac ABSORPTION_RWT >>
+  fs[FLOOKUP_DEF]);
+
+val apply_action_preserves_FDOMs = store_thm(
+  "apply_action_preserves_FDOMs",
+  ``apply_action a (SOME(lm,gm)) = SOME (lm',gm') ⇒
+    FDOM lm' = FDOM lm ∧ FDOM gm' = FDOM gm``,
+  simp[apply_action_def] >>
+  `selapf a lm = (FST,ap1) ∨ selapf a lm = (SND, ap2)`
+    by rw[selapf_def] >>
+  simp[] >> metis_tac[updf_preserves_FDOMs]);
+
+val selapf_cases = store_thm(
+  "selapf_cases",
+  ``∀a lm. selapf a lm = (FST, ap1) ∨ selapf a lm = (SND, ap2)``,
+  rw[selapf_def]);
+
+val updf_preserves_array_presence_length_back = store_thm(
+  "updf_preserves_array_presence_length_back",
+  ``updf w value m = SOME m' ∧ FLOOKUP m' a = SOME (Array els) ⇒
+    ∃els'. FLOOKUP m a = SOME (Array els') ∧ LENGTH els' = LENGTH els``,
+  simp[updf_def] >> Cases_on `w` >> simp[] >| [
+    simp[upd_array_def] >> Cases_on `FLOOKUP m s` >> simp[] >>
+    Cases_on `x` >> simp[] >> rw[] >> fs[FLOOKUP_DEF]
+    >- (rw[] >> fs[] >> rw[]) >>
+    Cases_on `a = s` >> fs[FAPPLY_FUPDATE_THM] >> rw[],
+    rw[FLOOKUP_DEF] >> Cases_on `m ' s` >>
+    fs[] >> rw[] >> fs[] >> rw[] >> fs[] >>
+    Cases_on `a = s` >> fs[FAPPLY_FUPDATE_THM]
+  ]);
+
+val updf_preserves_array_presence_length_forward = store_thm(
+  "updf_preserves_array_presence_length_forward",
+  ``updf w value m = SOME m' ∧ FLOOKUP m a = SOME (Array els) ⇒
+    ∃els'. FLOOKUP m' a = SOME (Array els') ∧ LENGTH els' = LENGTH els``,
+  simp[updf_def] >> Cases_on `w` >> simp[] >| [
+    simp[upd_array_def] >> Cases_on `FLOOKUP m s` >> simp[] >>
+    Cases_on `x` >> simp[] >> rw[] >> fs[FLOOKUP_DEF] >>
+    Cases_on `a = s` >> fs[FAPPLY_FUPDATE_THM] >> rw[],
+    rw[FLOOKUP_DEF] >> Cases_on `m ' s` >> fs[] >> rw[] >> fs[] >>
+    rw[] >> fs[] >>
+    Cases_on `a = s` >> fs[FAPPLY_FUPDATE_THM]
+  ]);
+
+val m_t = ``m:memory``
+val m'_t = ``m':memory``
+
+val nontouching_updfs_read_after_write = store_thm(
+  "nontouching_updfs_read_after_write",
+  ``updf w value m = SOME m' ∧ w ≠ rd ⇒ lookupRW m' rd = lookupRW m rd``,
+  `(∃a i. w = Array a i) ∨ ∃s. w = Variable s` by (Cases_on `w` >> simp[]) >>
+  `(∃b j. rd = Array b j) ∨ ∃t. rd = Variable t` by (Cases_on `rd` >> simp[]) >>
+  simp[updf_def, lookupRW_def, lookup_array_def, upd_array_def, lookup_v_def] >>
+  strip_tac
+  >- (`FLOOKUP m a = NONE ∨ ∃v. FLOOKUP m a = SOME v`
+        by (Cases_on `FLOOKUP m a` >> simp[]) >> fs[] >>
+      Cases_on `v` >> fs[FLOOKUP_DEF] >> rw[FAPPLY_FUPDATE_THM])
+  >- (`FLOOKUP m a = NONE ∨ ∃v. FLOOKUP m a = SOME v`
+        by (Cases_on `FLOOKUP m a` >> simp[]) >> fs[] >>
+      Cases_on `v` >> fs[FLOOKUP_DEF] >> rw[FAPPLY_FUPDATE_THM]
+      >- (rw[] >>
+          `0 ≤ i ∧ 0 ≤ j` by ARITH_TAC >>
+          `i = &(Num i) ∧ j = &(Num j)`
+            by metis_tac[integerTheory.INT_OF_NUM] >>
+          `Num j < LENGTH l`
+              by (fs[integerTheory.INT_NOT_LE] >>
+                  metis_tac[integerTheory.INT_LT]) >>
+          simp[listTheory.LUPDATE_SEM] >>
+          metis_tac[integerTheory.INT_INJ])
+      >- fs[]
+      >- fs[])
+  >- (`FLOOKUP m a = NONE ∨ ∃v. FLOOKUP m a = SOME v`
+        by (Cases_on `FLOOKUP m a` >> simp[]) >> fs[] >>
+      Cases_on `v` >> fs[FLOOKUP_DEF] >> rw[FAPPLY_FUPDATE_THM] >>
+      fs[])
+  >- (`FLOOKUP m s = NONE ∨ ∃v. FLOOKUP m s = SOME v`
+        by (Cases_on `FLOOKUP m s` >> simp[]) >> fs[] >>
+      Cases_on `v` >> fs[FLOOKUP_DEF] >> rw[FAPPLY_FUPDATE_THM] >>
+      fs[] >> Cases_on `value` >> fs[])
+  >- (`FLOOKUP m s = NONE ∨ ∃v. FLOOKUP m s = SOME v`
+        by (Cases_on `FLOOKUP m s` >> simp[]) >> fs[] >>
+      Cases_on `v` >> fs[FLOOKUP_DEF] >> rw[FAPPLY_FUPDATE_THM] >>
+      fs[] >> Cases_on `value` >> fs[]))
+
+val nontouching_updfs_varread_after_write = store_thm(
+  "nontouching_updfs_varread_after_write",
+  ``updf w value m = SOME m' ∧ actRWName w ≠ s ⇒ m' ' s = m ' s``,
+  `(∃a i. w = Array a i) ∨ ∃t. w = Variable t` by (Cases_on `w` >> simp[]) >>
+  simp[updf_def, lookupRW_def, lookup_array_def, upd_array_def, lookup_v_def] >>
+  strip_tac
+  >- (`FLOOKUP m a = NONE ∨ ∃v. FLOOKUP m a = SOME v`
+        by (Cases_on `FLOOKUP m a` >> simp[]) >> fs[] >>
+      Cases_on `v` >> fs[FLOOKUP_DEF] >> rw[FAPPLY_FUPDATE_THM])
+  >- (`FLOOKUP m t = NONE ∨ ∃v. FLOOKUP m t = SOME v`
+        by (Cases_on `FLOOKUP m t` >> simp[]) >> fs[] >>
+      Cases_on `v` >> fs[FLOOKUP_DEF] >> rw[FAPPLY_FUPDATE_THM]));
+
+val lookupRW_FUNION_L = store_thm(
+  "lookupRW_FUNION_L",
+  ``lookupRW m1 r = lookupRW m2 r ∧ FDOM m1 = FDOM m2 ⇒
+    lookupRW (m1 ⊌ m) r = lookupRW (m2 ⊌ m) r``,
+  Cases_on `r` >>
+  rw[lookupRW_def, lookup_array_def, lookup_v_def, FLOOKUP_DEF, FUNION_DEF] >>
+  fs[]);
+
+val lookupRW_FUNION_R = store_thm(
+  "lookupRW_FUNION_R",
+  ``lookupRW m1 r = lookupRW m2 r ∧ FDOM m1 = FDOM m2 ⇒
+    lookupRW (m ⊌ m1) r = lookupRW (m ⊌ m2) r``,
+  Cases_on `r` >>
+  rw[lookupRW_def, lookup_array_def, lookup_v_def, FLOOKUP_DEF, FUNION_DEF] >>
+  fs[]);
+
+
+val nontouching_updfs_expreval_L = store_thm(
+  "nontouching_updfs_expreval_L",
+  ``¬(touches a1 a2) ∧ updf a2.write value m = SOME m' ⇒
+    MAP (lookupRW (m' ⊌ m0)) a1.reads = MAP (lookupRW (m ⊌ m0)) a1.reads``,
+  simp[listTheory.MAP_EQ_f] >> strip_tac >> qx_gen_tac `r` >>
+  strip_tac >> match_mp_tac lookupRW_FUNION_L >>
+  `r ≠ a2.write` by metis_tac[touches_def] >>
+  metis_tac[nontouching_updfs_read_after_write, updf_preserves_FDOMs]);
+
+val nontouching_updfs_expreval_R = store_thm(
+  "nontouching_updfs_expreval_R",
+  ``¬(touches a1 a2) ∧ updf a2.write value m = SOME m' ⇒
+    MAP (lookupRW (m0 ⊌ m')) a1.reads = MAP (lookupRW (m0 ⊌ m)) a1.reads``,
+  simp[listTheory.MAP_EQ_f] >> strip_tac >> qx_gen_tac `r` >> strip_tac >>
+  match_mp_tac lookupRW_FUNION_R >>
+  `r ≠ a2.write` by metis_tac[touches_def] >>
+  metis_tac[nontouching_updfs_read_after_write, updf_preserves_FDOMs]);
+
+val FLOOKUP_memory_cases = prove(
+  ``!x: value option.
+      x = NONE ∨ (∃i. x = SOME (Int i)) ∨ (∃r. x = SOME (Real r)) ∨
+      (∃vl. x = SOME (Array vl)) ∨ (∃b. x = SOME (Bool b)) ∨
+      x = SOME Error``,
+  metis_tac[optionTheory.option_CASES, TypeBase.nchotomy_of ``:value``]);
+
+fun findOptionCases (g as (asl,w)) =
+    case bvk_find_term
+           (fn (bvs,t) => optionSyntax.is_option (type_of t) andalso
+                          HOLset.isEmpty
+                            (HOLset.intersection(
+                                HOLset.fromList Term.compare bvs,
+                                FVL [t] empty_tmset)) andalso
+                          not (optionSyntax.is_none t) andalso
+                          not (optionSyntax.is_some t)
+                          andalso
+                          not (can (find_term is_abs) t))
+           (fn x => x) w
+    of
+       NONE => NO_TAC g
+     | SOME t => Cases_on `^t` g
+
+val NEQ_SOME = prove(
+  ``x = NONE ⇒ x ≠ SOME y``,
+  simp[])
+
+val selapf_t = ``selapf a1 m``
+fun resolve_selapfs (g as (asl,w)) = let
+  val sel_t = find_term (can (match_term selapf_t)) w
+in
+  case List.find (fn t => aconv (rator (lhs t)) (rator sel_t)) asl of
+      NONE => NO_TAC
+    | SOME asm_t => SUBGOAL_THEN (mk_eq(sel_t, lhs asm_t)) ASSUME_TAC >| [
+                      REWRITE_TAC [selapf_def] >> AP_THM_TAC >> AP_THM_TAC >>
+                      AP_TERM_TAC >> AP_TERM_TAC >> RES_TAC,
+                      ALL_TAC
+                    ]
+end g
+
+val flookupmem_t = ``FLOOKUP (m:memory) s``
+val matches_flookupmem = can (match_term flookupmem_t)
+fun flookupmem_tac (g as (asl,w)) = let
+  val t = find_term matches_flookupmem w
+in
+  STRIP_ASSUME_TAC (SPEC t FLOOKUP_memory_cases) g
+end
+
+fun asmflookupmem_tac (g as (asl,w)) = let
+  fun flmem_subt t =
+      bvk_find_term (fn (bvs,t) => null bvs andalso matches_flookupmem t)
+                    (fn x => x) t
+in
+  case get_first flmem_subt asl of
+      NONE => NO_TAC g
+    | SOME t => STRIP_ASSUME_TAC (SPEC t FLOOKUP_memory_cases) g
+end
+
+fun eqNONE_tac (g as (asl,w)) = let
+  val asm_eqNONE_t =
+      valOf (List.find (fn t => is_eq t andalso
+                                type_of (rhs t) = ``:memory option`` andalso
+                                optionSyntax.is_none (rhs t))
+                       asl) handle Option => raise mk_HOL_ERR "" "" ""
+  val upd_t = #1 (strip_comb (lhs asm_eqNONE_t))
+  val upd_name = #1 (dest_var upd_t)
+  val other_name = if upd_name = "A1U" then "A2U" else "A1U"
+  val rearrange_tac =
+      case List.find (fn t => is_eq t andalso
+                              type_of (rhs t) = ``:memory option`` andalso
+                              optionSyntax.is_some (rhs t) andalso
+                              aconv upd_t (#1 (strip_comb (lhs t)))) asl
+       of
+          NONE => ALL_TAC
+        | SOME t => UNDISCH_TAC t >> CONV_TAC (REWR_CONV IMP_DISJ_THM) >>
+                    disj1_tac >> match_mp_tac NEQ_SOME
+  val flookup_case =
+    gen_tac >>
+    rpt strip_tac >>
+    qunabbrev_tac [QUOTE other_name] >> fs[] >>
+    first_x_assum (fn th10 => let
+      val th1 =
+          assert (can (match_term ``updf WW VV MM = SOME MM'`` o concl))
+                 th10
+    in
+      pop_assum (fn th2 =>
+        let
+          val th =
+              MATCH_MP (GEN_ALL updf_preserves_array_presence_length_forward)
+                       (CONJ th1 th2)
+              handle HOL_ERR _ =>
+              MATCH_MP (GEN_ALL updf_preserves_array_presence_length_back)
+                       (CONJ th1 th2)
+        in
+          STRIP_ASSUME_TAC th
+        end)
+    end) >>
+    pop_assum (fn th1 =>
+      pop_assum (fn th2 =>
+        first_x_assum (fn imp =>
+          mp_tac (SPEC (rand (rand (rhs (concl th2)))) imp)) >>
+        assume_tac th2) >>
+      assume_tac th1) >> simp[]
+  val expr_case =
+    disj2_tac >> disj1_tac >>
+    qpat_assum `XX = Array ZZ:value`
+      (fn th => EXISTS_TAC (rand (rhs (concl th))) THEN
+                REWRITE_TAC [SYM th]) >> AP_TERM_TAC >>
+    simp[listTheory.MAP_EQ_f] >> rpt strip_tac >>
+    (match_mp_tac lookupRW_FUNION_L ORELSE
+     match_mp_tac lookupRW_FUNION_R) >> ASM_REWRITE_TAC [] >>
+    qunabbrev_tac [QUOTE other_name] >> fs[] >>
+    metis_tac[nontouching_updfs_read_after_write, touches_def]
+  val vararray_case =
+    disj2_tac >> qunabbrev_tac [QUOTE other_name] >> fs[] >>
+    qpat_assum `vv ∈ FDOM (mm:memory)`
+      (fn th => let
+         val m_t = rand (rand (concl th))
+       in
+         assume_tac th >>
+         qpat_assum `updf ww vv ^m_t = SOME mm'`
+           (fn th => Cases_on `^(hd (#2 (strip_comb (lhs (concl th)))))` >>
+                     mp_tac th)
+       end) >> simp[updf_def, upd_array_def] >>
+    flookupmem_tac >> simp[] >> rw[] >>
+    rw[FAPPLY_FUPDATE_THM] >>
+    fs[touches_def, FAPPLY_FUPDATE_THM, FLOOKUP_DEF] >>
+    full_simp_tac (srw_ss() ++ boolSimps.COND_elim_ss) [] >> fs[]
+  val None_subtac = flookup_case ORELSE expr_case ORELSE vararray_case
+in
+  rearrange_tac >>
+  RES_TAC >>
+  qunabbrev_tac [QUOTE upd_name] >>
+  fs[updf_EQ_NONE, updarray_EQ_NONE] >>
+  None_subtac
+end g
+
+val updf_VAR_SOME_EQN = store_thm(
+  "updf_VAR_SOME_EQN",
+  ``updf (Variable s) v m = SOME m' ⇔
+    (∀es. v ≠ Array es) ∧ s ∈ FDOM m ∧ (∀es. m ' s ≠ Array es) ∧
+    m' = m |+ (s,v)``,
+  simp[updf_def] >> flookupmem_tac >> simp[] >> fs[FLOOKUP_DEF] >>
+  metis_tac[]);
+
+val updf_writes_commute = store_thm(
+  "updf_writes_commute",
+  ``w1 ≠ w2 ∧
+    updf w1 v1 m0 = SOME m11 ∧ updf w2 v2 m11 = SOME m12 ∧
+    updf w2 v2 m0 = SOME m21 ∧ updf w1 v1 m21 = SOME m22 ⇒
+    m12 = m22``,
+  Cases_on `w1` >> Cases_on `w2` >| [
+    simp[updf_def, upd_array_def] >>
+    rpt (flookupmem_tac >> simp[]) >> rw[] >>
+    fs[FLOOKUP_DEF, FAPPLY_FUPDATE_THM, integerTheory.INT_NOT_LE,
+       integerTheory.INT_NOT_LT] >|
+    [
+      dsimp[fmap_EXT, FAPPLY_FUPDATE_THM] >> conj_tac
+      >- (simp[EXTENSION] >> metis_tac[]) >>
+      rw[],
+      rw[] >> dsimp[fmap_EXT, FAPPLY_FUPDATE_THM] >> csimp[] >>
+      qmatch_rename_tac `
+        LUPDATE v2 (Num j) (LUPDATE v1 (Num i) a1) =
+        LUPDATE v1 (Num i) (LUPDATE v2 (Num j) a2)` [] >>
+      `a1 = a2` by fs[] >> rw[] >>
+      simp[listTheory.LIST_EQ_REWRITE, listTheory.LUPDATE_SEM] >>
+      `Num i ≠ Num j`
+        by metis_tac[integerTheory.INT_INJ, integerTheory.INT_OF_NUM] >>
+      rw[] >> fs[],
+      qmatch_rename_tac `
+        m0 |+ (s, Array (LUPDATE v1 (Num i) a1))
+           |+ (t, Array (LUPDATE v2 (Num j) a2)) = XX` ["XX"] >>
+      reverse (Cases_on `s = t`)
+      >- (fs[] >> dsimp[fmap_EXT, FAPPLY_FUPDATE_THM] >>
+          rw[EXTENSION] >> metis_tac[]) >>
+      fs[] >> rw[] >> dsimp[fmap_EXT, FAPPLY_FUPDATE_THM] >> csimp[] >>
+      `Num i ≠ Num j`
+        by metis_tac[integerTheory.INT_INJ, integerTheory.INT_OF_NUM] >>
+      simp[listTheory.LIST_EQ_REWRITE, listTheory.LUPDATE_SEM] >>
+      rw[] >> fs[]
+    ],
+
+    simp[SPEC ``Array a i`` updf_def, upd_array_def,
+         updf_VAR_SOME_EQN] >>
+    rpt (flookupmem_tac >> simp[]) >> fs[FLOOKUP_DEF] >>
+    rpt strip_tac >> rw[] >>
+    qmatch_rename_tac `m0 |+ (s, XX) |+ (t, YY) = ZZ`
+      ["XX", "YY", "ZZ"] >>
+    `s ≠ t` by (strip_tac >> fs[]) >>
+    fs[FAPPLY_FUPDATE_THM] >> metis_tac[FUPDATE_COMMUTES],
+
+    simp[SPEC ``Array a i`` updf_def, upd_array_def,
+         updf_VAR_SOME_EQN] >>
+    rpt (flookupmem_tac >> simp[]) >> fs[FLOOKUP_DEF] >>
+    rpt strip_tac >> rw[] >>
+    qmatch_rename_tac `m0 |+ (s, XX) |+ (t, YY) = ZZ`
+      ["XX", "YY", "ZZ"] >>
+    `s ≠ t` by (strip_tac >> fs[]) >>
+    fs[FAPPLY_FUPDATE_THM] >> metis_tac[FUPDATE_COMMUTES],
+
+    simp[updf_VAR_SOME_EQN] >> rpt strip_tac >>
+    simp[FUPDATE_COMMUTES]
+  ])
+
+fun ae_equate_tac anm (g as (asl,w)) = let
+  fun ae_term t = let
+    val (f, xs) = strip_comb t
+  in
+    #1 (dest_var f) = "ae" andalso length xs = 2 andalso
+    #1 (dest_var (hd xs)) = anm
+  end handle HOL_ERR _ => false
+  fun get_ae_term t =
+      bvk_find_term (fn (_,t) => ae_term t) (fn x => x) t
+  val (t1,t2) = case List.mapPartial get_ae_term asl of
+                    [t1,t2] => (t1,t2)
+                  | _ => raise mk_HOL_ERR "" "ae_equate_tac"
+                               ("Don't have 2 ae-terms for "^anm)
+in
+  SUBGOAL_THEN (mk_eq(t1,t2)) SUBST_ALL_TAC THENL [
+    qunabbrev_tac `ae` >> fs[] >>
+    metis_tac[nontouching_updfs_expreval_R, touches_SYM,
+              nontouching_updfs_expreval_L],
+    ALL_TAC
+  ]
+end g
+
+val success_case =
+  rpt (qpat_assum `selapf xx yy = zz` kall_tac) >>
+  rpt (first_x_assum (kall_tac o assert (is_forall o concl))) >>
+  map_every qunabbrev_tac [`A1U`, `A2U`] >> fs[] >>
+  qabbrev_tac `
+    ae = λa:(value,actionRW,α)action m. a.expr (MAP (lookupRW m) a.reads)
+  ` >> fs[] >>
+  ae_equate_tac "a1" >> ae_equate_tac "a2" >> fs[] >>
+  metis_tac[updf_writes_commute, touches_def]
+
+
+val apply_action_commutes = store_thm(
+  "apply_action_commutes",
+  ``¬(a1:(value,actionRW,α)action ∼ₜ a2:(value,actionRW,α)action) ⇒
+    (apply_action a2 (apply_action a1 m) =
+     apply_action a1 (apply_action a2 m))``,
+  strip_tac >>
+  `m = NONE ∨ ∃lm gm. m = SOME(lm,gm)`
+     by metis_tac[optionTheory.option_CASES, pairTheory.pair_CASES] >>
+  simp[apply_action_def, lift_OPTION_BIND, combinTheory.o_ABS_R,
+       pairTheory.o_UNCURRY_R, pairTheory.C_UNCURRY_L,
+       combinTheory.C_ABS_L] >>
+  qabbrev_tac `A1U = λm. updf a1.write (a1.expr (MAP (lookupRW m) a1.reads))` >>
+  qabbrev_tac `A2U = λm. updf a2.write (a2.expr (MAP (lookupRW m) a2.reads))` >>
+  simp[] >>
+  `(∀rm m m'. A1U rm m = SOME m' ⇒ FDOM m' = FDOM m) ∧
+   (∀rm m m'. A2U rm m = SOME m' ⇒ FDOM m' = FDOM m)`
+     by (simp[Abbr`A1U`, Abbr`A2U`] >> metis_tac[updf_preserves_FDOMs]) >>
+  Q.ISPECL_THEN [`a1`, `lm`] strip_assume_tac selapf_cases >>
+  Q.ISPECL_THEN [`a2`, `lm`] strip_assume_tac selapf_cases >>
+  fs[] >> rw[] >>
+  rpt (findOptionCases >> simp[]) >>
+  rpt (resolve_selapfs >> simp[]) >> TRY eqNONE_tac >>
+  rpt (findOptionCases >> simp[]) >> TRY eqNONE_tac >>
+  success_case)
 
 val graphOf_def = tDefine "graphOf" `
 
@@ -271,9 +747,9 @@ val graphOf_def = tDefine "graphOf" `
      do (aname,i_e) <- SOME w;
         i <- (some i. evalexpr (lm0 ⊌ m0) i_e = Int i);
         rds <- getReads (lm0 ⊌ m0) ds;
-        a <- SOME <| write := (aname,i);
+        a <- SOME <| write := Array aname i;
                      reads := rds;
-                     expr := mergeReads (lm0 ⊌ m0) ds opn;
+                     expr := mergeReads ds opn;
                      iter := iter |> ;
         rvs <- OPT_SEQUENCE (MAP (evalDexpr (lm0 ⊌ m0)) ds);
         m' <- upd_array m0 aname i (opn rvs);
